Interop wrappers for inline fmul, fmul2, fsqr, fsqr2

vale/code/arch/x64/interop/Fmul_inline.fst
@@ -38,6 +38,281 @@ let t64_no_mod = TD_Buffer TUInt64 TUInt64 ({modified=false; strict_disjointness
 [@__reduce__] unfold
 let tuint64 = TD_Base TUInt64
 
+
+[@__reduce__] unfold
+let fmul_dom: IX64.arity_ok 4 td =
+  let y = [t64_mod; t64_no_mod; t64_mod; t64_no_mod] in
+  assert_norm (List.length y = 4);
+  y
+
+(* Need to rearrange the order of arguments *)
+[@__reduce__]
+let fmul_pre : VSig.vale_pre 48 fmul_dom =
+  fun (c:V.va_code)
+    (tmp:b64)
+    (f1:b64)
+    (out:b64)
+    (f2:b64)
+    (va_s0:V.va_state)
+    (sb:IX64.stack_buffer 48) ->
+      FW.va_req_fmul c va_s0 (as_vale_buffer sb) 
+        (as_vale_buffer tmp) (as_vale_buffer f1) (as_vale_buffer out) (as_vale_buffer f2)
+
+[@__reduce__]
+let fmul_post : VSig.vale_post 48 fmul_dom =
+  fun (c:V.va_code)
+    (tmp:b64)
+    (f1:b64)
+    (out:b64)
+    (f2:b64)
+    (va_s0:V.va_state)
+    (sb:IX64.stack_buffer 48)
+    (va_s1:V.va_state)
+    (f:V.va_fuel) ->
+      FW.va_ens_fmul c va_s0 (as_vale_buffer sb) (as_vale_buffer tmp) (as_vale_buffer f1) (as_vale_buffer out) (as_vale_buffer f2) va_s1 f
+
+let fmul_regs_modified: MS.reg -> bool = fun (r:MS.reg) ->
+  let open MS in
+  if r = Rax || r = Rcx || r = Rdx || r = Rdi || r = Rsi || r = R8 || r = R9 || r = R10 || r = R11 || r = R12 || r = R13 || r = R14 || r = R15 then true
+  else false
+
+let fmul_xmms_modified = fun _ -> false
+
+#set-options "--z3rlimit 200"
+
+[@__reduce__] unfold
+let fmul_lemma'
+    (code:V.va_code)
+    (_win:bool)
+    (tmp:b64)
+    (f1:b64)
+    (out:b64)
+    (f2:b64)
+    (va_s0:V.va_state)
+    (sb:IX64.stack_buffer 48)
+ : Ghost (V.va_state & V.va_fuel)
+     (requires
+       fmul_pre code tmp f1 out f2 va_s0 sb)
+     (ensures (fun (va_s1, f) ->
+       V.eval_code code va_s0 f va_s1 /\
+       VSig.vale_calling_conventions va_s0 va_s1 fmul_regs_modified fmul_xmms_modified /\
+       fmul_post code tmp f1 out f2 va_s0 sb va_s1 f /\
+       ME.buffer_readable VS.(va_s1.mem) (as_vale_buffer out) /\
+       ME.buffer_readable VS.(va_s1.mem) (as_vale_buffer f1) /\ 
+       ME.buffer_readable VS.(va_s1.mem) (as_vale_buffer f2) /\ 
+       ME.buffer_readable VS.(va_s1.mem) (as_vale_buffer tmp) /\ 
+       ME.buffer_writeable (as_vale_buffer out) /\ 
+       ME.buffer_writeable (as_vale_buffer f1) /\
+       ME.buffer_writeable (as_vale_buffer f2) /\       
+       ME.buffer_writeable (as_vale_buffer tmp) /\       
+       ME.modifies (ME.loc_union (ME.loc_buffer (as_vale_buffer sb))
+                   (ME.loc_union (ME.loc_buffer (as_vale_buffer out))
+                   (ME.loc_union (ME.loc_buffer (as_vale_buffer tmp))
+                                 ME.loc_none))) va_s0.VS.mem va_s1.VS.mem
+ )) = 
+   let va_s1, f = FW.va_lemma_fmul code va_s0 (as_vale_buffer sb) (as_vale_buffer tmp) (as_vale_buffer f1) (as_vale_buffer out) (as_vale_buffer f2) in
+   Vale.AsLowStar.MemoryHelpers.buffer_writeable_reveal ME.TUInt64 ME.TUInt64 out;   
+   Vale.AsLowStar.MemoryHelpers.buffer_writeable_reveal ME.TUInt64 ME.TUInt64 f1;   
+   Vale.AsLowStar.MemoryHelpers.buffer_writeable_reveal ME.TUInt64 ME.TUInt64 f2;   
+   Vale.AsLowStar.MemoryHelpers.buffer_writeable_reveal ME.TUInt64 ME.TUInt64 tmp;       
+   va_s1, f                                   
+
+(* Prove that fmul_lemma' has the required type *)
+let fmul_lemma = as_t #(VSig.vale_sig fmul_regs_modified fmul_xmms_modified fmul_pre fmul_post) fmul_lemma'
+let code_fmul = FW.va_code_fmul ()
+
+let fmul_of_reg (r:MS.reg) : option (IX64.reg_nat 4) = match r with
+  | MS.Rdi -> Some 0
+  | MS.Rsi -> Some 1
+  | MS.Rdx -> Some 2
+  | MS.Rcx -> Some 3
+  | _ -> None
+
+let fmul_of_arg (i:IX64.reg_nat 4) = match i with
+  | 0 -> MS.Rdi
+  | 1 -> MS.Rsi
+  | 2 -> MS.Rdx
+  | 3 -> MS.Rcx
+
+let fmul_arg_reg : IX64.arg_reg_relation 4 = IX64.Rel fmul_of_reg fmul_of_arg
+
+(* Here's the type expected for the fmul wrapper *)
+[@__reduce__] noextract
+let lowstar_fmul_t =
+  assert_norm (List.length fmul_dom + List.length ([]<:list arg) <= 4);
+  IX64.as_lowstar_sig_t_weak
+    4
+    fmul_arg_reg
+    fmul_regs_modified
+    fmul_xmms_modified
+    Interop.down_mem
+    code_fmul
+    48
+    fmul_dom
+    []
+    _
+    _
+    (W.mk_prediction code_fmul fmul_dom [] (fmul_lemma code_fmul IA.win))
+
+(* And here's the fmul wrapper itself *)
+let lowstar_fmul : lowstar_fmul_t  =
+  assert_norm (List.length fmul_dom + List.length ([]<:list arg) <= 4);
+  IX64.wrap_weak
+    4
+    fmul_arg_reg
+    fmul_regs_modified
+    fmul_xmms_modified
+    Interop.down_mem
+    code_fmul
+    48
+    fmul_dom
+    (W.mk_prediction code_fmul fmul_dom [] (fmul_lemma code_fmul IA.win))
+
+let lowstar_fmul_normal_t : normal lowstar_fmul_t
+  = as_normal_t #lowstar_fmul_t lowstar_fmul
+
+open Vale.AsLowStar.MemoryHelpers
+
+#push-options "--max_fuel 0 --max_ifuel 0 --z3rlimit 200"
+
+let math_aux (n:nat) : Lemma ((n*8)/8 = n) = ()
+
+let fmul_inline tmp f1 out f2 =
+    DV.length_eq (get_downview out);
+    DV.length_eq (get_downview f1);
+    DV.length_eq (get_downview tmp);
+    DV.length_eq (get_downview f2);
+    math_aux (B.length tmp);
+    math_aux (B.length out);
+    Vale.AsLowStar.MemoryHelpers.as_vale_buffer_len #TUInt64 #TUInt64 tmp;
+    Vale.AsLowStar.MemoryHelpers.as_vale_buffer_len #TUInt64 #TUInt64 out;    
+    let x, _ = lowstar_fmul_normal_t tmp f1 out f2 () in
+    ()
+
+#pop-options
+
+let fmul_code_inline () : FStar.All.ML int =
+  PR.print_inline "fmul" 0 None (List.length fmul_dom) fmul_dom code_fmul fmul_of_arg fmul_regs_modified
+
+(* Need to rearrange the order of arguments *)
+[@__reduce__]
+let fmul2_pre : VSig.vale_pre 48 fmul_dom =
+  fun (c:V.va_code)
+    (tmp:b64)
+    (f1:b64)
+    (out:b64)
+    (f2:b64)
+    (va_s0:V.va_state)
+    (sb:IX64.stack_buffer 48) ->
+      FW.va_req_fmul2 c va_s0 (as_vale_buffer sb) 
+        (as_vale_buffer tmp) (as_vale_buffer f1) (as_vale_buffer out) (as_vale_buffer f2)
+
+[@__reduce__]
+let fmul2_post : VSig.vale_post 48 fmul_dom =
+  fun (c:V.va_code)
+    (tmp:b64)
+    (f1:b64)
+    (out:b64)
+    (f2:b64)
+    (va_s0:V.va_state)
+    (sb:IX64.stack_buffer 48)
+    (va_s1:V.va_state)
+    (f:V.va_fuel) ->
+      FW.va_ens_fmul2 c va_s0 (as_vale_buffer sb) (as_vale_buffer tmp) (as_vale_buffer f1) (as_vale_buffer out) (as_vale_buffer f2) va_s1 f
+
+#set-options "--z3rlimit 200"
+
+[@__reduce__] unfold
+let fmul2_lemma'
+    (code:V.va_code)
+    (_win:bool)
+    (tmp:b64)
+    (f1:b64)
+    (out:b64)
+    (f2:b64)
+    (va_s0:V.va_state)
+    (sb:IX64.stack_buffer 48)
+ : Ghost (V.va_state & V.va_fuel)
+     (requires
+       fmul2_pre code tmp f1 out f2 va_s0 sb)
+     (ensures (fun (va_s1, f) ->
+       V.eval_code code va_s0 f va_s1 /\
+       VSig.vale_calling_conventions va_s0 va_s1 fmul_regs_modified fmul_xmms_modified /\
+       fmul2_post code tmp f1 out f2 va_s0 sb va_s1 f /\
+       ME.buffer_readable VS.(va_s1.mem) (as_vale_buffer out) /\
+       ME.buffer_readable VS.(va_s1.mem) (as_vale_buffer f1) /\ 
+       ME.buffer_readable VS.(va_s1.mem) (as_vale_buffer f2) /\ 
+       ME.buffer_readable VS.(va_s1.mem) (as_vale_buffer tmp) /\ 
+       ME.buffer_writeable (as_vale_buffer out) /\ 
+       ME.buffer_writeable (as_vale_buffer f1) /\
+       ME.buffer_writeable (as_vale_buffer f2) /\       
+       ME.buffer_writeable (as_vale_buffer tmp) /\       
+       ME.modifies (ME.loc_union (ME.loc_buffer (as_vale_buffer sb))
+                   (ME.loc_union (ME.loc_buffer (as_vale_buffer out))
+                   (ME.loc_union (ME.loc_buffer (as_vale_buffer tmp))
+                                 ME.loc_none))) va_s0.VS.mem va_s1.VS.mem
+ )) = 
+   let va_s1, f = FW.va_lemma_fmul2 code va_s0 (as_vale_buffer sb) (as_vale_buffer tmp) (as_vale_buffer f1) (as_vale_buffer out) (as_vale_buffer f2) in
+   Vale.AsLowStar.MemoryHelpers.buffer_writeable_reveal ME.TUInt64 ME.TUInt64 out;   
+   Vale.AsLowStar.MemoryHelpers.buffer_writeable_reveal ME.TUInt64 ME.TUInt64 f1;   
+   Vale.AsLowStar.MemoryHelpers.buffer_writeable_reveal ME.TUInt64 ME.TUInt64 f2;   
+   Vale.AsLowStar.MemoryHelpers.buffer_writeable_reveal ME.TUInt64 ME.TUInt64 tmp;      
+   va_s1, f                                   
+
+(* Prove that fmul2_lemma' has the required type *)
+let fmul2_lemma = as_t #(VSig.vale_sig fmul_regs_modified fmul_xmms_modified fmul2_pre fmul2_post) fmul2_lemma'
+let code_fmul2 = FW.va_code_fmul2 ()
+
+(* Here's the type expected for the fmul wrapper *)
+[@__reduce__]
+let lowstar_fmul2_t =
+  assert_norm (List.length fmul_dom + List.length ([]<:list arg) <= 4);
+  IX64.as_lowstar_sig_t_weak
+    4
+    fmul_arg_reg
+    fmul_regs_modified
+    fmul_xmms_modified
+    Interop.down_mem
+    code_fmul2
+    48
+    fmul_dom
+    []
+    _
+    _
+    (W.mk_prediction code_fmul2 fmul_dom [] (fmul2_lemma code_fmul2 IA.win))
+
+(* And here's the fmul2 wrapper itself *)
+let lowstar_fmul2 : lowstar_fmul2_t  =
+  assert_norm (List.length fmul_dom + List.length ([]<:list arg) <= 4);
+  IX64.wrap_weak
+    4
+    fmul_arg_reg
+    fmul_regs_modified
+    fmul_xmms_modified
+    Interop.down_mem
+    code_fmul2
+    48
+    fmul_dom
+    (W.mk_prediction code_fmul2 fmul_dom [] (fmul2_lemma code_fmul2 IA.win))
+
+let lowstar_fmul2_normal_t : normal lowstar_fmul2_t
+  = as_normal_t #lowstar_fmul2_t lowstar_fmul2
+
+#push-options "--max_fuel 0 --max_ifuel 0 --z3rlimit 200"
+
+let fmul2_inline tmp f1 out f2 =
+    DV.length_eq (get_downview out);
+    DV.length_eq (get_downview f1);
+    DV.length_eq (get_downview tmp);
+    DV.length_eq (get_downview f2);
+    let x, _ = lowstar_fmul2_normal_t tmp f1 out f2 () in
+    ()
+
+#pop-options
+
+let fmul2_code_inline () : FStar.All.ML int =
+  PR.print_inline "fmul2" 0 None (List.length fmul_dom) fmul_dom code_fmul2 fmul_of_arg fmul_regs_modified
+
 [@__reduce__] unfold
 let fmul1_dom: IX64.arity_ok 3 td =
   let y = [t64_mod; t64_no_mod; tuint64] in
