vale/code/arch/x64/interop/Fmul_inline.fsti
@@ -22,54 +22,52 @@ let as_nat (b:B.buffer UInt64.t{B.length b == 4}) (h:HS.mem) : GTot nat =
   let s3 = UInt64.v (Seq.index s 3) in
   pow2_four s0 s1 s2 s3
 
-// No definition that is not stdcall for these two
+val fmul_inline
+  (tmp:u512)
+  (f1:u256)
+  (out:u256) 
+  (f2:u256)
+  : Stack unit
+    (requires fun h -> 
+      adx_enabled /\ bmi2_enabled /\
+      B.live h out /\ B.live h f1 /\ B.live h f2 /\ B.live h tmp /\
+      (B.disjoint out f1 \/ out == f1) /\
+      (B.disjoint out f2 \/ out == f2) /\
+      (B.disjoint out tmp \/ out == tmp) /\
+      (B.disjoint f1 f2 \/ f1 == f2) /\
+      B.disjoint f1 tmp /\
+      B.disjoint f2 tmp
+    )
+    (ensures  fun h0 _ h1 ->
+      B.modifies (B.loc_union (B.loc_buffer out) (B.loc_buffer tmp)) h0 h1 /\
+      (as_nat out h1) % prime == (as_nat f1 h0 * as_nat f2 h0) % prime)
 
-// val fmul_inline
-//   (tmp:u512)
-//   (f1:u256)
-//   (out:u256) 
-//   (f2:u256)
-//   : Stack unit
-//     (requires fun h -> 
-//       adx_enabled /\ bmi2_enabled /\
-//       B.live h out /\ B.live h f1 /\ B.live h f2 /\ B.live h tmp /\
-//       (B.disjoint out f1 \/ out == f1) /\
-//       (B.disjoint out f2 \/ out == f2) /\
-//       (B.disjoint out tmp \/ out == tmp) /\
-//       (B.disjoint f1 f2 \/ f1 == f2) /\
-//       B.disjoint f1 tmp /\
-//       B.disjoint f2 tmp
-//     )
-//     (ensures  fun h0 _ h1 ->
-//       B.modifies (B.loc_union (B.loc_buffer out) (B.loc_buffer tmp)) h0 h1 /\
-//       (as_nat out h1) % prime == (as_nat f1 h0 * as_nat f2 h0) % prime)
-
-// val fmul2_inline
-//   (tmp:u1024)
-//   (f1:u512)
-//   (out:u512) 
-//   (f2:u512)
-//   : Stack unit
-//     (requires fun h -> 
-//       adx_enabled /\ bmi2_enabled /\
-//       B.live h out /\ B.live h f1 /\ B.live h f2 /\ B.live h tmp /\
-//       (B.disjoint out f1 \/ out == f1) /\
-//       (B.disjoint out f2 \/ out == f2) /\
-//       (B.disjoint out tmp \/ out == tmp) /\
-//       (B.disjoint f1 f2 \/ f1 == f2) /\
-//       B.disjoint f1 tmp /\
-//       B.disjoint f2 tmp
-//     )
-//     (ensures  fun h0 _ h1 ->
-//       B.modifies (B.loc_union (B.loc_buffer out) (B.loc_buffer tmp)) h0 h1 /\
-//      (let out0 = B.gsub out 0ul 4ul in
-//       let out1 = B.gsub out 4ul 4ul in
-//       let f10 = B.gsub f1 0ul 4ul in
-//       let f11 = B.gsub f1 4ul 4ul in
-//       let f20 = B.gsub f2 0ul 4ul in
-//       let f21 = B.gsub f2 4ul 4ul in
-//       (as_nat out0 h1) % prime == (as_nat f10 h0 * as_nat f20 h0) % prime /\
-//       (as_nat out1 h1) % prime == (as_nat f11 h0 * as_nat f21 h0) % prime))
+val fmul2_inline
+  (tmp:u1024)
+  (f1:u512)
+  (out:u512) 
+  (f2:u512)
+  : Stack unit
+    (requires fun h -> 
+      adx_enabled /\ bmi2_enabled /\
+      B.live h out /\ B.live h f1 /\ B.live h f2 /\ B.live h tmp /\
+      (B.disjoint out f1 \/ out == f1) /\
+      (B.disjoint out f2 \/ out == f2) /\
+      (B.disjoint out tmp \/ out == tmp) /\
+      (B.disjoint f1 f2 \/ f1 == f2) /\
+      B.disjoint f1 tmp /\
+      B.disjoint f2 tmp
+    )
+    (ensures  fun h0 _ h1 ->
+      B.modifies (B.loc_union (B.loc_buffer out) (B.loc_buffer tmp)) h0 h1 /\
+     (let out0 = B.gsub out 0ul 4ul in
+      let out1 = B.gsub out 4ul 4ul in
+      let f10 = B.gsub f1 0ul 4ul in
+      let f11 = B.gsub f1 4ul 4ul in
+      let f20 = B.gsub f2 0ul 4ul in
+      let f21 = B.gsub f2 4ul 4ul in
+      (as_nat out0 h1) % prime == (as_nat f10 h0 * as_nat f20 h0) % prime /\
+      (as_nat out1 h1) % prime == (as_nat f11 h0 * as_nat f21 h0) % prime))
 
 val fmul1_inline
   (out:u256)
